store.v
@@ -1,0 +1,501 @@
+From stdpp Require Import base gmap.
+From mathcomp Require Import ssreflect.
+From stdpp Require Import namespaces.
+From iris.algebra Require Import agree auth csum gset gmap excl frac.
+From iris.algebra Require Import max_prefix_list.
+From iris.heap_lang Require Import notation proofmode.
+From cryptis Require Import lib term cryptis primitives tactics.
+From cryptis Require Import role session pk_auth pk_dh.
+
+Set Implicit Arguments.
+Unset Strict Implicit.
+Unset Printing Implicit Defensive.
+
+(* MOVE *)
+#[global]
+Instance if_persistent (Σ : gFunctors) (b : bool) (φ ψ : iProp Σ) :
+  Persistent φ →
+  Persistent ψ →
+  Persistent (if b then φ else ψ).
+Proof. by case: b. Qed.
+(* /MOVE *)
+
+Record cst := {
+  cst_ts   : loc;
+  cst_key  : term;
+  cst_name : gname;
+  cst_ok   : bool;
+}.
+
+#[local]
+Instance cst_repr : Repr cst := λ s, (#(cst_ts s), Spec.mkskey (cst_key s))%V.
+
+(* FIXME: Maybe generalize this *)
+Definition sess_recv N : val := λ: "c" "k" "f",
+  do_until (λ: <>,
+    let: "m" := recv "c" in
+    bind: "m" := tsdec N "k" "m" in
+    "f" "m"
+  ).
+
+Module Client.
+
+Section Client.
+
+Variable N : namespace.
+
+Definition connect : val := λ: "c" "skA" "pkA" "pkB",
+  do_until (λ: <>,
+    bind: "kS" := pk_dh_init N "c" "skA" "pkA" "pkB" in
+    let: "l"  := ref #0 in
+    let: "kS" := mkskey (tag (N.@"key") "kS") in
+    SOME ("l", "kS")
+  ).
+
+Definition get_ts : val := λ: "cs",
+  let: "l" := Fst "cs" in
+  !"l".
+
+Definition next_ts : val := λ: "cs",
+  let: "l" := Fst "cs" in
+  "l" <- (!"l" + #1).
+
+Definition get_sk : val := λ: "cs",
+  Snd "cs".
+
+Definition send_store : val := λ: "c" "cs" "v",
+  next_ts "cs";;
+  let: "n" := get_ts "cs" in
+  let: "sk" := get_sk "cs" in
+  let: "m" := tsenc (N.@"store") "sk" (term_of_list [tint "n"; "v"]) in
+  send "c" "m".
+
+Definition ack_store : val := λ: "c" "cs",
+  let: "n" := get_ts "cs" in
+  let: "sk" := get_sk "cs" in
+  sess_recv (N.@"ack_store") "c" "sk" (λ: "m",
+    assert: eq_term "m" (tint "n") in
+    SOME #()
+  ).
+
+Definition store : val := λ: "c" "cs" "t",
+  send_store "c" "cs" "t";;
+  ack_store "c" "cs".
+
+Definition load : val := λ: "c" "cs",
+  let: "n" := tint (get_ts "cs") in
+  let: "sk" := get_sk "cs" in
+  send "c" (tsenc (N.@"load") "sk" "n");;
+  sess_recv (N.@"ack_load") "c" "sk" (λ: "resp",
+    bind: "resp" := list_of_term "resp" in
+    list_match: ["n'"; "t"] := "resp" in
+    assert: eq_term "n'" "n" in
+    SOME "t"
+  ).
+
+End Client.
+
+End Client.
+
+Record sst := {
+  sst_ts  : loc;
+  sst_val : loc;
+  sst_key : term;
+}.
+
+#[global]
+Instance repr_sst : Repr sst :=
+  λ ss, (#(sst_ts ss), #(sst_val ss), sst_key ss)%V.
+
+Module Server.
+
+Implicit Types N : namespace.
+
+Definition get_ts : val := λ: "ss",
+  !(Fst "ss").
+
+Definition set_ts : val := λ: "ss" "ts",
+  Fst "ss" <- "ts".
+
+Definition get_val : val := λ: "ss",
+  !(Fst (Snd "ss")).
+
+Definition set_val : val := λ: "ss" "v",
+  Fst (Snd "ss") <- "v".
+
+Definition get_key : val := λ: "ss",
+  Snd (Snd "ss").
+
+Definition handle_store N : val := λ: "c" "ss" "m",
+  bind: "m" := list_of_term "m" in
+  list_match: ["n"; "x"] := "m" in
+  bind: "n'" := to_int "n" in
+  assert: get_ts "ss" ≤ "n'" in
+  set_ts "ss" "n'";;
+  set_val "ss" "v";;
+  send "c" (tenc (N.@"ack_store") (get_key "ss") "n").
+
+Definition handle_load N : val := λ: "c" "ss" "m",
+  bind: "n" := to_int "m" in
+  assert: get_ts "ss" = "n" in
+  let: "v" := get_val "ss" in
+  send "c" (tsenc (N.@"ack_load") (get_key "ss") (term_of_list ["m"; "v"])).
+
+Definition conn_handler_body N : val := λ: "c" "ss",
+  let: "sk" := get_key "ss" in
+  let: "m" := recv "c" in
+  match: tsdec (N.@"store") "sk" "m" with
+    SOME "m" => handle_store N "c" "ss" "m"
+  | NONE => match: tsdec (N.@"load") "sk" "m" with
+    SOME "m" => handle_load N "c" "ss" "m"
+  | NONE => #()
+  end end.
+
+Definition conn_handler N : val := rec: "loop" "c" "ss" :=
+  conn_handler_body N "c" "ss";;
+  "loop" "c" "ss".
+
+Definition listen N : val := rec: "loop" "c" "skB" "pkB" :=
+  match: pk_dh_resp N "c" "skB" "pkB" with
+    NONE =>
+    "loop" "c" "skB" "pkB"
+  | SOME "res" =>
+    let: "pkA" := Fst "res" in
+    let: "kS"  := mkskey (tag (N.@"key") (Snd "res")) in
+    let: "ss"  := (ref #0, ref #0, "ks") in
+    Fork (conn_handler N "c" "ss");;
+    "loop" "c" "skB" "pkB"
+  end.
+
+End Server.
+
+Section Verif.
+
+Context `{!cryptisG Σ, !heapGS Σ, !sessionG Σ}.
+Notation iProp := (iProp Σ).
+
+Class storeG := StoreG {
+  store_inG :> inG Σ (authR (max_prefix_listUR termO));
+}.
+
+Context `{!storeG}.
+
+Local Instance STORE : PK := PK_DH (λ _ _ _ _, True)%I.
+
+Implicit Types s : cst.
+Implicit Types kI kR kS t : term.
+Implicit Types n : nat.
+Implicit Types γ : gname.
+Implicit Types cs v : val.
+
+(* FIXME: infer the invariant φ in a tactic, similarly to how iLöb works *)
+Lemma wp_sess_recv E N c sk (f : val) φ Φ Ψ :
+  ↑cryptisN ⊆ E →
+  channel c -∗
+  enc_pred N Φ -∗
+  sterm sk -∗
+  □ (∀ t,
+      φ -∗
+      ▷ (pterm (TKey Enc sk) ∗ pterm t ∨
+         sterm t ∗ □ Φ sk t ∗ □ (pterm (TKey Dec sk) → pterm t)) -∗
+      WP f t @ E {{ v, ⌜v = NONEV⌝ ∗ φ ∨ ∃ v', ⌜v = SOMEV v'⌝ ∗ Ψ v' }}) -∗
+  φ -∗ WP sess_recv N c (Spec.mkskey sk) f @ E {{ Ψ }}.
+Proof.
+iIntros "% #chan_c #ΦP #s_sk #wp_f Hφ"; rewrite /sess_recv; wp_pures.
+iRevert "Hφ". iApply wp_do_until; iIntros "!> Hφ". wp_pures.
+wp_bind (recv _); iApply wp_recv => //.
+iIntros "%t #p_t"; wp_pures.
+wp_tsdec_eq t' e; wp_pures; eauto.
+rewrite {}e {t} pterm_TEnc.
+iApply ("wp_f" with "Hφ"). rewrite pterm_tag.
+iDestruct "p_t" as "[[??] | p_t]"; eauto.
+iRight. rewrite sterm_TEnc sterm_tag.
+iDestruct "p_t" as "[[??] [inv_t' p_t]]".
+do 2![iSplit => //].
+iPoseProof (wf_enc_elim with "inv_t' ΦP") as "{inv_t'} #inv_t'".
+eauto.
+Qed.
+
+Variable N : namespace.
+
+Definition cur_term_auth γ n t : iProp := ∃ ts,
+  own γ (● to_max_prefix_list (ts ++ [t]) ⋅
+         ◯ to_max_prefix_list (ts ++ [t])) ∗
+  ⌜n = length ts⌝.
+
+Definition cur_term_frag γ n t : iProp := ∃ ts,
+  own γ (◯ to_max_prefix_list (ts ++ [t])) ∗
+  ⌜n = length ts⌝.
+
+Lemma cur_term_auth_alloc : ⊢ |==> ∃ γ, cur_term_auth γ 0 (TInt 0).
+Proof.
+iMod (own_alloc (● to_max_prefix_list [TInt 0] ⋅
+                 ◯ to_max_prefix_list [TInt 0])) as "[%γ own]".
+  rewrite auth_both_valid_discrete; split; eauto.
+  by apply to_max_prefix_list_valid.
+iModIntro. iExists γ, []. rewrite /=. iFrame. by eauto.
+Qed.
+
+#[global]
+Instance cur_term_frag_persistent γ n t : Persistent (cur_term_frag γ n t).
+Proof. apply _. Qed.
+
+Lemma cur_term_auth_frag γ n t : cur_term_auth γ n t -∗ cur_term_frag γ n t.
+Proof.
+iDestruct 1 as "(%ts & [own1 #own2] & %nE)".
+iExists ts; eauto.
+Qed.
+
+Lemma upd_cur_term γ n t t' :
+  cur_term_auth γ n t ==∗ cur_term_auth γ (n + 1) t'.
+Proof.
+iDestruct 1 as "(%ts & own & ->)".
+iMod (own_update with "own") as "own".
+  eapply auth_update.
+  apply (max_prefix_list_local_update _ ((ts ++ [t]) ++ [t'])).
+  by exists [t'].
+iModIntro. rewrite plus_comm /=.
+iExists (ts ++ [t]). rewrite own_op app_length. iFrame.
+iPureIntro. simpl. lia.
+Qed.
+
+Definition store_key kI kR kS γ : iProp := ∃ kS',
+  ⌜kS = Spec.tag (N.@"key") kS'⌝ ∗
+  pk_dh_session_meta N (λ _ _ _ _, True)%I Init kI kR kS' N γ ∗
+  □ (∀ kt, pterm (TKey kt kS) -∗ ◇ False).
+
+Definition client_state kI kR s n t : iProp :=
+  cst_ts s ↦ #n ∗
+  sterm (cst_key s) ∗
+  cur_term_auth (cst_name s) n t ∗
+  if cst_ok s then store_key kI kR (cst_key s) (cst_name s)
+  else corruption kI kR.
+
+Lemma client_state_cur_term_frag kI kR s n t :
+  client_state kI kR s n t -∗
+  cur_term_frag (cst_name s) n t.
+Proof.
+iIntros "(_ & _ & ? & _)".
+by iApply cur_term_auth_frag.
+Qed.
+
+Lemma client_state_cst_key kI kR s n t :
+  client_state kI kR s n t -∗
+  sterm (cst_key s) ∗
+  if cst_ok s then store_key kI kR (cst_key s) (cst_name s)
+  else corruption kI kR.
+Proof. by iIntros "(_ & ? & _ & ?)"; eauto. Qed.
+
+Definition store_pred kS m : iProp := ∃ (n : nat) t kI kR γ,
+  ⌜m = Spec.of_list [TInt n; t]⌝ ∗
+  cur_term_frag γ n t ∗
+  (corruption kI kR ∨ store_key kI kR kS γ).
+
+Definition ack_store_pred kS m : iProp := ∃ (n : nat),
+  ⌜m = TInt n⌝. (* FIXME: Do we need anything else here? *)
+
+Definition load_pred (kS m : term) : iProp := True.
+
+Definition ack_load_pred kS m : iProp := ∃ (n : nat) t,
+  ⌜m = Spec.of_list [TInt n; t]⌝ ∗
+  ∀ kI kR γ t', store_key kI kR kS γ -∗
+  cur_term_frag γ n t' -∗
+  ⌜t = t'⌝.
+
+Definition ctx : iProp :=
+  enc_pred (N.@"store") store_pred ∗
+  enc_pred (N.@"ack_store") ack_store_pred ∗
+  enc_pred (N.@"load") load_pred ∗
+  enc_pred (N.@"ack_load") ack_load_pred ∗
+  pk_dh_ctx N (λ _ _ _ _, True)%I ∗
+  key_pred (N.@"key") (λ _ _, False)%I.
+
+Lemma wp_client_get_ts E kI kR s n t :
+  {{{ client_state kI kR s n t }}}
+    Client.get_ts (repr s) @ E
+  {{{ RET #n; client_state kI kR s n t }}}.
+Proof.
+rewrite /Client.get_ts.
+iIntros "%Φ (Hl & #s_kS & Hγ & state) post".
+wp_pures. wp_load. iApply "post". iModIntro. by iFrame.
+Qed.
+
+Lemma wp_client_next_ts t' E kI kR s n t :
+  {{{ client_state kI kR s n t }}}
+    Client.next_ts (repr s) @ E
+  {{{ RET #(); client_state kI kR s (n + 1) t' }}}.
+Proof.
+iIntros "%Ψ (n_stored & #s_key & n_t & auth) post".
+iMod (upd_cur_term _ _ _ t' with "n_t") as "n_t".
+rewrite /Client.next_ts; wp_pures; wp_load; wp_store.
+iApply "post"; iFrame.
+rewrite (_ : (n + 1)%nat = (n + 1)%Z :> Z); last by lia.
+by iFrame.
+Qed.
+
+Lemma wp_client_get_sk E kI kR s n t :
+  {{{ client_state kI kR s n t }}}
+    Client.get_sk (repr s) @ E
+  {{{ RET (repr (Spec.mkskey (cst_key s))); client_state kI kR s n t }}}.
+Proof.
+rewrite /Client.get_sk.
+iIntros "%Φ ? post". wp_pures. by iApply "post".
+Qed.
+
+Lemma wp_client_send_store E kI kR c s n t t' :
+  ↑cryptisN ⊆ E →
+  channel c -∗
+  ctx -∗
+  pterm t' -∗ (* FIXME: t' does not have to be public already *)
+  {{{ client_state kI kR s n t }}}
+    Client.send_store N c (repr s) t' @ E
+  {{{ RET #(); client_state kI kR s (n + 1) t' }}}.
+Proof.
+rewrite /Client.send_store.
+iIntros "% #chan_c (#? & _) #p_t' !> %Φ state post".
+wp_pures. wp_bind (Client.next_ts _).
+iApply (wp_client_next_ts t' with "state"); iIntros "!> state".
+iPoseProof (client_state_cur_term_frag with "state") as "#frag".
+wp_pures. wp_bind (Client.get_ts _).
+iApply (wp_client_get_ts with "state"); iIntros "!> state".
+wp_pures. wp_bind (Client.get_sk _).
+iApply (wp_client_get_sk with "state"); iIntros "!> state".
+iPoseProof (client_state_cst_key with "state") as "# (s_k & p_k)".
+wp_pures. wp_list. wp_bind (tint _). iApply wp_tint. wp_list.
+wp_term_of_list. wp_tsenc. wp_pures.
+iApply (wp_send with "[//]"); eauto; last by iApply "post".
+iModIntro. iApply pterm_TEncIS => //.
+- by rewrite sterm_TKey.
+- iModIntro. iExists (n + 1), t', kI, kR, (cst_name s).
+  rewrite Nat2Z.inj_add /=.
+  iSplit => //. iSplit => //. by case: (cst_ok s); eauto.
+- rewrite sterm_of_list /= sterm_TInt; do ![iSplit => //].
+  by iApply pterm_sterm.
+- iModIntro. iIntros "_". rewrite pterm_of_list /= pterm_TInt. iSplit => //.
+  by iSplit => //.
+Qed.
+
+Lemma wp_client_ack_store E kI kR c s n t :
+  ↑cryptisN ⊆ E →
+  channel c -∗
+  ctx -∗
+  {{{ client_state kI kR s n t }}}
+    Client.ack_store N c (repr s) @ E
+  {{{ RET #(); client_state kI kR s n t }}}.
+Proof.
+iIntros "% #chan_c (_ & #? & _) !> %Φ state post".
+rewrite /Client.ack_store. wp_pures.
+wp_bind (Client.get_ts _). iApply (wp_client_get_ts with "state") => //.
+iIntros "!> state". wp_pures.
+wp_bind (Client.get_sk _). iApply (wp_client_get_sk with "state") => //.
+iIntros "!> state". wp_pures.
+iPoseProof (client_state_cst_key with "state") as "#[s_k ?]".
+iCombine "post state" as "I". iRevert "I".
+iApply wp_sess_recv => //. iIntros "!> %m [post state] _".
+wp_pures. wp_bind (tint _). iApply wp_tint.
+wp_eq_term e; wp_pures; iModIntro; last first.
+  iLeft. by iFrame.
+iRight. iExists _; iSplit => //. by iApply "post".
+Qed.
+
+Lemma wp_client_store E kI kR c s n t t' :
+  ↑cryptisN ⊆ E →
+  channel c -∗
+  ctx -∗
+  pterm t' -∗
+  {{{ client_state kI kR s n t }}}
+    Client.store N c (repr s) t' @ E
+  {{{ RET #(); client_state kI kR s (n + 1) t' }}}.
+Proof.
+iIntros "% #chan_c #ctx #p_t' !> %Φ state post". rewrite /Client.store.
+wp_pures. wp_bind (Client.send_store _ _ _ _).
+iApply (wp_client_send_store with "[] [] [] [state] [post]") => //.
+iIntros "!> state". wp_pures.
+iApply (wp_client_ack_store with "[] [] [state] [post]") => //.
+Qed.
+
+Lemma wp_client_connect E c kI kR :
+  ↑N ⊆ E →
+  ↑cryptisN ⊆ E →
+  channel c -∗
+  ctx -∗
+  pterm (TKey Enc kI) -∗
+  pterm (TKey Enc kR) -∗
+  {{{ True }}}
+    Client.connect N c (TKey Dec kI) (TKey Enc kI) (TKey Enc kR) @ E
+  {{{ s, RET (repr s); client_state kI kR s 0 (TInt 0) }}}.
+Proof.
+iIntros "% % #chan_c (_ & _ & _ & _ & #ctx & #key) #p_ekI #p_ekR".
+iIntros "!> %Φ _ post". rewrite /Client.connect. wp_pures.
+iRevert "post". iApply wp_do_until. iIntros "!> post". wp_pures.
+wp_bind (pk_dh_init _ _ _ _ _).
+iApply (wp_pk_dh_init with "[] [] [] [] []"); eauto.
+iIntros "!> %okS HokS". case: okS => [kS|]; wp_pures; last by iLeft; eauto.
+wp_alloc l as "Hl". wp_pures. wp_tag. wp_bind (mkskey _). iApply wp_mkskey.
+iMod cur_term_auth_alloc as "[%γ cur_term]".
+wp_pures. iRight. iExists _. iSplitR; eauto.
+iDestruct "HokS" as "(#s_kS & _ & status)".
+rewrite [(_ ∨ _)%I]comm bi.or_alt. iDestruct "status" as "(%ok & status)".
+iApply ("post" $! {| cst_ts := l; cst_key := Spec.tag (N.@"key") kS;
+                     cst_name := γ; cst_ok := ok |}).
+rewrite /client_state /=. iFrame. rewrite sterm_tag.
+iSplitR => //.
+case: ok; last by eauto.
+iDestruct "status" as "(#p_kS & token & #session)".
+iMod (term_meta_set _ _ γ N with "token") as "#meta"; eauto.
+iModIntro. iExists kS. do 2!iSplit => //. iIntros "!> %kt #p_kS'".
+rewrite (pterm_TKey kt) pterm_tag sterm_tag.
+iDestruct "p_kS'" as "[?|[_ p_kS']]"; first by iApply "p_kS".
+by iMod (wf_key_elim with "p_kS' key") as "#[]".
+Qed.
+
+Lemma wp_client_load E c kI kR s n t :
+  ↑N ⊆ E →
+  ↑cryptisN ⊆ E →
+  channel c -∗
+  ctx -∗
+  pterm (TKey Enc kI) -∗
+  pterm (TKey Enc kR) -∗
+  {{{ client_state kI kR s n t }}}
+    Client.load N c (repr s) @ E
+  {{{ t', RET (repr t');
+      client_state kI kR s n t ∗
+      ◇ ⌜cst_ok s → t' = t⌝ }}}.
+Proof.
+iIntros "% % #chan_c #ctx #p_ekI #p_ekR !> %Φ state post".
+iDestruct "ctx" as "(_ & _ & ? & ? & _)".
+rewrite /Client.load. wp_pures.
+wp_bind (Client.get_ts _). iApply (wp_client_get_ts with "state").
+iIntros "!> state". wp_pures. wp_bind (tint _). iApply wp_tint.
+wp_pures. wp_bind (Client.get_sk _).
+iApply (wp_client_get_sk with "state"). iIntros "!> state". wp_pures.
+wp_tsenc. wp_pures.
+iPoseProof (client_state_cst_key with "state") as "#[s_k status]".
+wp_bind (send _ _). iApply wp_send; eauto.
+  iModIntro. iApply pterm_TEncIS; eauto.
+  - by rewrite sterm_TKey.
+  - by rewrite sterm_TInt.
+  - rewrite pterm_TInt. by eauto.
+wp_pures.
+iCombine "post state" as "I". iRevert "I". iApply wp_sess_recv => //.
+iIntros "!> %ts [post state] #p_t'". wp_pures.
+wp_list_of_term ts; wp_pures; last by iLeft; iFrame.
+wp_list_match => [n' v -> {ts}|_]; wp_pures; last by iLeft; iFrame.
+wp_eq_term e; wp_pures; last by iLeft; iFrame.
+subst n'. iModIntro. iRight. iExists _; iSplit; eauto.
+iApply ("post" $! v). iSplit => //.
+case e_ok: (cst_ok s) => //=. iIntros "_".
+iPoseProof "status" as "(%kS' & %e_kS & #meta & #p_kS)".
+iDestruct "p_t'" as "[[contra _] | succ]".
+  iMod ("p_kS" $! Enc with "contra") as "{contra} #[]".
+iDestruct "succ" as "(_ & #wf_t' & _)".
+iDestruct "wf_t'" as "(%n' & %t' & %e & tP)".
+iDestruct "state" as "(_ & _ & auth & _)".
+case/Spec.of_list_inj: e => /Nat2Z.inj <- <- {n' t'}.
+iModIntro.
+iApply "tP".
+- by iApply "status".
+- by iApply cur_term_auth_frag.
+Qed.
+
+End Verif.
